Test.fst
@@ -1,13 +1,50 @@
 module Test
 
+
 open FStar.Tactics
 
-let empty = _:unit{False}
-let g : unit -> bool = fun x -> true
-let h : unit -> bool = fun x -> false
-let gh (x:empty) : Lemma(g x == h x) = ()
+let e_wp (a:Type) : Type = nat -> Type0
+let e_repr (a:Type) (w:e_wp a) : Type = _:a{w 5}
 
-let unsound () : Lemma(False) =
-  assert ((fun (x:empty) -> g x) == (fun (x:empty) -> h x)) by (l_to_r [`gh]); // by substituting
-  assert (g == h);  // by eta-reduction
-  assert (g () == h ())
+assume val ew_return (a:Type) (x:a) : e_wp a
+assume val e_return (a:Type) (x:a) : e_repr a (ew_return a x)
+
+assume val ew_bind (a b:Type) (w1:e_wp a) (w2:a->e_wp b) : e_wp b
+assume val e_bind (a b:Type) (w1:e_wp a) (w2:a->e_wp b)       (f: e_repr a w1) (g: (x:a -> e_repr b (w2 x))) : e_repr b (ew_bind a b w1 w2)
+
+total
+reflectable
+reifiable
+layered_effect { E : (a:Type) -> (wp:e_wp a) -> Effect with 
+  repr = e_repr;
+  return = e_return; 
+  bind = e_bind
+//  subcomp = prob_subcomp;
+//  if_then_else = ite_prob
+  }
+
+
+let e1 #a : e_wp a = (fun _ -> True) 
+let e2 #a : e_wp a = (fun n -> n==5) 
+
+let ew_lift a (wp:pure_wp a) = e1 #a
+
+let e_lift a (wp:pure_wp a) (f: eqtype_as_type unit -> PURE a wp) : 
+   e_repr a (ew_lift a wp) =
+   admit()
+   
+
+sub_effect PURE ~> E = e_lift
+
+
+let also_type (#a #b #b': Type) (#wp1:a -> e_wp b) (p:(x:a) -> E b (wp1 x)) (wp2:a -> e_wp b') = unit -> q:(x:a -> E b' (wp2 x)) {forall(x:a). reify (p x) === reify (q x)}
+ 
+let test () : E unit e1 = E?.reflect ()
+
+let test_also : also_type test (fun () -> e2 #unit) = 
+  fun () ->
+  let p' = reify (test ()) in
+  let q : unit -> E unit e2 = (fun x -> E?.reflect p') in
+  assert (reify (test ()) === reify (q ())) by ();
+  q
+
